LTSb.thy
@@ -1,0 +1,221 @@
+theory LTSb
+
+imports Main
+
+begin
+
+section {* Labeled transition systems and their executions *}
+
+subsection {* Labeled transition systems *}
+
+text {* 
+  The semantics of a B component is a discrete, eventful, state-transition system. We 
+  formalize labeled transition systems (LTS) and their behaviors, independently of B.
+  An LTS is given by a set of initial states and a set of transitions, which are
+  triples (source and destination state, and a transition label). The following
+  definitions of transitions and transition systems are parameterized by types
+  @{text "'st"} and @{text "'ev"} of states and events.
+*}
+
+record ('st, 'ev) Tr =
+  src :: 'st     -- "source state"
+  dst :: 'st     -- "destination state"
+  lbl :: 'ev     -- "labeling event"
+
+record ('st, 'ev) LTS =
+  init :: "'st set" -- "set of initial states"
+  trans :: "('st, 'ev) Tr set" -- "set of transitions"
+
+text {*
+   We first introduce auxiliary definitions for some useful
+   concepts. The function @{text "outgoing"}, given a LTS and a
+   state, returns the set of outgoing transitions in that state.  
+*}
+
+definition
+  outgoing :: "('st, 'ev) LTS \<Rightarrow> 'st \<Rightarrow> ('st, 'ev) Tr set"
+where
+  "outgoing l \<equiv> \<lambda>s. { t | t . t \<in> trans l \<and> src t = s}"
+
+text {*
+  The function @{text "accepted_events"}, given an LTS and a state,
+  returns the set of events that label the outgoing transitions in
+  that state. It corresponds to the operations and the corresponding
+  parameter valuations that are applicable in that state.  
+*}
+
+definition
+  accepted_events :: "('st, 'ev) LTS \<Rightarrow> 'st \<Rightarrow> 'ev set"
+where
+  "accepted_events l s \<equiv> lbl ` (outgoing l s)"
+
+text {* 
+  The inductively defined set @{term "states m"} corresponds to the set of
+  reachable states of a given LTS @{text m}. 
+*}
+
+inductive_set states :: "('st, 'ev) LTS \<Rightarrow> 'st set" 
+  for l :: "('st, 'ev) LTS" where
+  base[elim!]: "s \<in> init l \<Longrightarrow> s \<in> states l"
+| step[elim!]: "\<lbrakk>s \<in> states l; t \<in> outgoing l s\<rbrakk> \<Longrightarrow> dst t \<in> states l"
+
+inductive_cases base : "s \<in> states l"
+inductive_cases step : "dst t \<in> states l"
+
+text {* 
+  A few lemmas related to reachable states are then enunciated and proved. 
+  First, all the initial states are reachable states:
+*}
+
+lemma reachable_init: "init l \<subseteq> states l"
+  by auto
+
+text {* Next, the successors states of the reachable states are themselves reachable states.
+We first define a function @{text "successors"} that returns the set of successors of a
+given set @{text "S"} of states in a given LTS @{text "l"}: *}
+
+definition successors :: "('st, 'ev) LTS \<Rightarrow> 'st set \<Rightarrow> 'st set" where
+  "successors l S \<equiv> dst ` (UNION S (outgoing l))"
+
+text {* Next, we show that the successors of the reachable states are also reachable. *}
+
+lemma reachable_stable: "successors l (states l) \<subseteq> states l"
+  unfolding successors_def by auto
+
+text {* 
+  The following lemma is at the basis of proofs of invariants, and more
+  generally, safety properties. Any set @{text S} that contains all initial
+  states and is closed under successors contains all reachable states.
+*}
+
+lemma reachable_induct_set:
+  assumes s: "s \<in> states l"
+  and "init l \<subseteq> S"
+  and "successors l S \<subseteq> S"
+  shows "s \<in> S"
+  using assms by (induct s) (auto simp: successors_def)
+
+text {*
+  The following lemma is similar but stated in terms of a predicate.
+  It contains the principle for proving invariants.
+*}
+lemmas reachable_induct_predicate = states.induct
+text {* @{thm reachable_induct_predicate} *}
+
+text {*
+  The \emph{alphabet} of an LTS is defined as the set of labels
+  appearing at some reachable state.
+*}
+
+definition alphabet where
+  "alphabet l \<equiv> UNION (states l) (accepted_events l)"
+
+
+subsection {* Behavior *}
+
+text {* 
+  Two views of (finitary) behavior are formalized. The first view is
+  the internal behavior: a \emph{run} is an initial state, followed by
+  an alternating sequence of events and states that correspond to
+  transitions of the LTS.
+
+  The second, external view of behavior, abstracts from the states and
+  only records the events that occur in a run.
+*}
+
+subsubsection {* Internal behaviour *}
+
+record ('st,'ev) Run =
+  trns :: "('st \<times> 'ev) list"
+  fins :: "'st"
+
+text {* 
+  The inductive set @{text "runs l"} denotes the set of finite executions
+  of the LTS @{text "l"}, viewed as lists of transitions. There are two base 
+  cases, corresponding to the empty execution and to executions with a 
+  single transition whose source state is an initial state.
+*}
+
+definition append_tr :: "('st,'ev) Run \<Rightarrow> ('st,'ev) Tr \<Rightarrow> ('st,'ev) Run" where
+  "append_tr run t \<equiv> \<lparr> trns = (trns run) @ [(fins run, lbl t)], fins = dst t \<rparr>"
+
+inductive_set runs :: "('st, 'ev) LTS \<Rightarrow> ('st, 'ev) Run set"  
+  for l :: "('st, 'ev) LTS" where
+  start: "s \<in> init l \<Longrightarrow> \<lparr> trns = [], fins = s \<rparr> \<in> runs l"
+| step : "\<lbrakk> run \<in> runs l; t \<in> outgoing l (fins run) \<rbrakk> \<Longrightarrow> append_tr run t \<in> runs l"
+
+text {* 
+  The following lemma states that every run starts in an initial state of @{text l}.
+*}
+
+lemma run_starts_initial: 
+  assumes "r \<in> runs l"
+  shows "(if trns r = [] then fins r else fst (hd (trns r))) \<in> init l"
+  using assms by (induct r, auto simp: append_tr_def hd_append)
+
+text {*
+  The set of runs is closed under prefixes.
+*}
+lemma prefix_is_run:
+  assumes "r \<in> runs l" and "n < length (trns r) - 1"
+  shows "\<lparr> trns = take n (trns r), fins = fst ((trns r)!n) \<rparr> \<in> runs l"
+proof -
+  {
+    fix r' t n'
+    assume r': "r' \<in> runs l"
+       and n': "n' < length (trns r')"
+       and t: "t \<in> outgoing l (fins r')"
+       and ih: "\<And>m. m < length (trns r') - Suc 0 \<Longrightarrow>
+                     \<lparr> trns = take m (trns r'),
+                       fins = fst (trns r' ! m) \<rparr> \<in> runs l"
+    have "\<lparr> trns = take n' (trns r'),
+            fins = fst ((trns r' @ [(fins r', lbl t)]) ! n')\<rparr> \<in> runs l"
+      (is "?run \<in> runs l")
+    proof (cases "n' < length (trns r') - Suc 0")
+      case True with ih n' show ?thesis
+        by (simp add: nth_append)
+    next
+      case False
+      with n' have len: "n' = length (trns r') - Suc 0" by auto
+      from r' show ?thesis
+      proof (cases r')
+        fix s
+        assume "r' = \<lparr> trns = [], fins = s \<rparr>"
+        with n' show ?thesis by auto  (* r' cannot be empty *)
+      next
+        fix r'' t'
+        assume r'': "r'' \<in> runs l"
+           and t': "t' \<in> outgoing l (fins r'')"
+           and r': "r' = append_tr r'' t'"
+        with len have "?run = r''" by (auto simp: append_tr_def)
+        with r'' show ?thesis by simp
+      qed
+    qed
+  }
+  with assms show ?thesis
+    by (induct r arbitrary: n, auto simp: append_tr_def)
+qed
+
+
+subsubsection {* External behavior. *}
+
+text {* 
+  The external, or observable, behavior of a LTS is obtained by
+  projecting the internal behavior to the events labeling its 
+  transitions. We call this a \emph{trace} of the LTS.
+*}
+
+type_synonym 'ev Trace = "'ev list"
+
+definition trace_of :: "('st, 'ev) Run \<Rightarrow> 'ev Trace" where
+  "trace_of run \<equiv> map snd (trns run)"
+
+lemma trace_of_length [simp]: 
+  "length (trace_of run) = length (trns run)"
+  unfolding trace_of_def by simp
+
+definition traces :: "('st, 'ev) LTS \<Rightarrow> 'ev Trace set" where
+  "traces l \<equiv> trace_of ` (runs l)"
+
+end
+
