Simulationb.thy
@@ -1,0 +1,169 @@
+theory Simulationb
+imports LTSb
+begin
+
+section {* Relating LTSes: simulation *}
+
+subsection {* Basic definitions *}
+
+text {* 
+  We formalize a notion of simulation on LTSes. Classic definitions of simulation
+  often consider a single LTS, and simulation is established between two states of the same
+  LTS. Here, a simulation is a relation @{text "r"} between the states of one LTS
+  and the states of another LTS such that any transition taken by the former can be simulated
+  by the latter. The development presented in this section aims to achieve the final theorem
+  that extends the simulation to full behavior, i.e. sequences of transitions.
+
+  The following function @{text "sim_transition"} lifts a relation on states to
+  a relation on transitions: it requires the source and destination states to be
+  related, and the labels to coincide.
+*}
+
+(* sm: should this notion be generalized to a relation between two possibly
+   distinct state types? *)
+definition sim_transition :: "'st rel \<Rightarrow> ('st, 'ev) Tr rel" where
+  "sim_transition r \<equiv> { (t,t') | t t'. (src t, src t') \<in> r
+                                     \<and> lbl t = lbl t' \<and> (dst t, dst t') \<in> r }"
+
+text {* 
+  A relation @{text r} on states induces a simulation relation over LTSes @{text l}
+  and @{text "l'"} if both of the following conditions hold:
+  \begin{itemize}
+  \item Every initial state of @{text l} is related to some initial state of @{text "l'"}.
+  \item For any states @{text "(s,s')"} related by @{text r} and any
+    transition @{text t} of @{text l} originating at @{text s} there exists a
+    transition of @{text "l'"} originating at @{text "s'"} that simulates @{text t}.
+  \end{itemize}
+*}
+
+definition simulation :: "'st rel \<Rightarrow> ('st, 'ev) LTS rel" where
+  "simulation r \<equiv> { (l,l') | l l'.
+     (\<forall>s \<in> init l. \<exists>s' \<in> init l'. (s, s') \<in> r)
+   \<and> (\<forall>s s'. (s, s') \<in> r \<longrightarrow>
+        (\<forall>t \<in> outgoing l s. \<exists>t' \<in> outgoing l' s'. (t,t') \<in> sim_transition r)) }"
+
+text {* 
+  We say that @{text "l'"} simulates @{text l} if is there is a simulation between
+  @{text l} and @{text "l'"}.
+*}
+definition simulated (infixl "\<preceq>" 50) where
+  "l \<preceq> l' \<equiv> \<exists>r. (l,l') \<in> simulation r"
+
+subsection {* Properties *}
+
+text {*
+  Let us verify some basic properties of simulations. First we have that
+  every LTS simulates itself, through a lifting of the identity relation
+  over states.
+*}
+
+lemma simulation_identity : "(Id::('st,'ev) LTS rel) \<subseteq> simulation (Id::'st rel)" 
+  unfolding simulation_def sim_transition_def by auto
+
+text {*
+   Second, we have that the composition of two simulation relations is a simulation relation.
+*}
+lemma simulation_composition:
+  assumes "(l, l') \<in> simulation r" and "(l', l'') \<in> simulation r'"
+  shows "(l, l'') \<in> simulation (r O r')"
+  using assms unfolding simulation_def sim_transition_def relcomp_unfold
+  by auto (metis+)
+
+text {* 
+  These properties are lifted to the simulates relation over LTS.
+*}
+
+lemma simulated_reflexive: "l \<preceq> l" 
+  unfolding simulated_def using simulation_identity by blast
+
+lemma simulated_transitive:
+  assumes "l \<preceq> l'" and "l' \<preceq> l''"
+  shows "l \<preceq> l''"
+  using assms unfolding simulated_def using simulation_composition by blast
+
+subsection {* Simulation and behavior *}
+
+text {*
+  Similarly, a relation @{text r} on states induces a simulation between two runs:
+  corresponding transitions must be related according to @{text r}, lifted to
+  transitions.
+*}
+definition sim_run :: "'st rel \<Rightarrow> ('st, 'ev) Run rel" where
+  "sim_run r \<equiv> {(run, run') | run run'. 
+                   length (trns run) = length (trns run')
+                 \<and> (\<forall>i < length (trns run). 
+                       (fst (trns run ! i), fst (trns run' ! i)) \<in> r
+                     \<and> snd (trns run ! i) = snd (trns run' ! i))
+                 \<and> (fins run, fins run') \<in> r}"
+
+text {* 
+  It immediately follows that two similar runs yield the same trace
+  (i.e., observable behavior).
+*}
+
+theorem sim_run_trace_eq: 
+  assumes "(run, run') \<in> sim_run r"
+  shows "trace_of run = trace_of run'"
+  using assms by (simp add: sim_run_def trace_of_def nth_equalityI)
+
+theorem sim_run:
+  assumes sim: "(l,l') \<in> simulation r" and run: "run \<in> runs l"
+  obtains run' where "run' \<in> runs l'" "(run,run') \<in> sim_run r"
+proof -
+  from run have "\<exists>run' \<in> runs l'. (run, run') \<in> sim_run r"
+  proof (induct)
+    fix s
+    assume "s \<in> init l"
+    with sim obtain s' where s': "s' \<in> init l'" "(s,s') \<in> r"
+      unfolding simulation_def by blast
+    hence "\<lparr> trns = [], fins = s' \<rparr> \<in> runs l'"
+      by (auto intro: runs.start)
+    with s' show "\<exists>run' \<in> runs l'. (\<lparr>trns = [], fins = s\<rparr>, run') \<in> sim_run r"
+      unfolding sim_run_def by force
+  next
+    fix rn t
+    assume rn: "rn \<in> runs l"
+       and ih: "\<exists>rn' \<in> runs l'. (rn, rn') \<in> sim_run r"
+       and t: "t \<in> outgoing l (fins rn)"
+    from ih obtain rn' where
+      rn': "rn' \<in> runs l'" "length (trns rn) = length (trns rn')"
+           "\<forall>i < length (trns rn).
+               (fst (trns rn ! i), fst (trns rn' ! i)) \<in> r
+             \<and> snd (trns rn ! i) = snd (trns rn' ! i)"
+           "(fins rn, fins rn') \<in> r"
+      unfolding sim_run_def by blast
+    with sim t obtain t' where
+      t': "t' \<in> outgoing l' (fins rn')" "lbl t' = lbl t" "(dst t, dst t') \<in> r"
+      unfolding simulation_def sim_transition_def by force
+    let ?run = "append_tr rn t"
+    let ?run' = "append_tr rn' t'"
+    from `rn' \<in> runs l'` `t' \<in> outgoing l' (fins rn')` have "?run' \<in> runs l'"
+      by (rule runs.step)
+    moreover
+    from rn' t' have "(?run, ?run') \<in> sim_run r"
+      unfolding sim_run_def by (auto simp: append_tr_def nth_append)
+    ultimately show "\<exists>run' \<in> runs l'. (?run, run') \<in> sim_run r" ..
+  qed
+  with that show ?thesis by blast
+qed
+
+lemma sim_traces:
+  assumes sim: "(l,l') \<in> simulation r" and tr: "tr \<in> traces l"
+  shows "tr \<in> traces l'"
+proof -
+  from tr obtain run where run: "run \<in> runs l" "tr = trace_of run"
+    by (auto simp: traces_def)
+  with sim obtain run' where "run' \<in> runs l'" "(run,run') \<in> sim_run r"
+    by (blast dest: sim_run)
+  with run show ?thesis
+    by (auto simp: traces_def sim_run_trace_eq)
+qed
+
+theorem sim_trace_inclusion: "(l,l') \<in> simulation r \<Longrightarrow> traces l \<subseteq> traces l'"
+  by (blast dest: sim_traces)
+
+corollary simulates_traces: "l \<preceq> l' \<Longrightarrow> traces l \<subseteq> traces l'"
+  unfolding simulated_def by (auto dest: sim_trace_inclusion)
+
+end
+
